Remove elaborate dependency for elaborate_record
This allows the corresponding proof to be simplified; however, the proof
of the lemma is still unfinished as the statement is missing an
assumption (which I haven't quite figured out how to state).

PyLevelLang/src/PyLevelLang/Elaborate.v
@@ -1,6 +1,6 @@
 Require Import PyLevelLang.Language.
 Require Import coqutil.Map.Interface coqutil.Map.SortedListString.
-Require Import coqutil.Datatypes.Result.
+Require Import coqutil.Datatypes.Result coqutil.Datatypes.List.
 Import ResultMonadNotations.
 
 (* Casts an expression `e` from `expr t2` to `expr t1`, if the two types are
@@ -63,6 +63,23 @@ Section WithMap.
   Proof.
     intros G H He.
     now apply enforce_type_pred with (e := e).
+  Qed.
+
+  Lemma existT_wf {t t'} (e : expr t) (e' : expr t') : forall G,
+    (existT expr t e = existT expr t' e') -> (wf G e -> wf G e').
+  Proof.
+    intros G H He.
+    destruct He; inversion H.
+    - apply wf_EVar.
+      now rewrite <- H2.
+    - apply wf_ELoc.
+      now rewrite <- H2.
+    - apply wf_EConst.
+    - now apply wf_EUnop.
+    - now apply wf_EBinop.
+    - now apply wf_EFlatmap.
+    - now apply wf_EIf.
+    - now apply wf_ELet.
   Qed.
 
   Definition elaborate_const (pc : pconst) : result {t & expr t} :=
@@ -259,6 +276,29 @@ Section WithMap.
       apply wf_EBinop; now apply enforce_type_wf with (G := G) in H2'.
   Qed.
 
+  Fixpoint elaborate_record (xs : list (string * {t & expr t})) :
+    result {t & expr t} :=
+    match xs with
+    | nil =>
+        Success (existT _ _ (EConst CEmpty))
+    | (s, (existT _ _ e1)) :: xs =>
+        '(existT _ _ e2) <- elaborate_record xs;;
+        Success (existT _ _ (EBinop (OPair s _ _) e1 e2))
+    end.
+
+  Lemma elaborate_record_wf (xs : list (string * {t & expr t})) : forall G t' e',
+    elaborate_record xs = Success (existT expr t' e') -> wf G e'.
+  Proof.
+    induction xs as [| [s [t1 e1]]]; intros G t' e' H.
+    - inversion H. apply wf_EConst.
+    - inversion H.
+      destruct elaborate_record as [[t2 e2] |]; try easy.
+      injection H1 as [= H2 H1].
+      apply existT_wf with (G := G) in H1; [easy | apply wf_EBinop].
+      + admit.
+      + now apply IHxs.
+  Admitted.
+
   Fixpoint elaborate_proj {t : type} (e : expr t) (s : string) :
     result {t & expr t} :=
     match t as t' return expr t' -> _ with
@@ -285,21 +325,6 @@ Section WithMap.
       + exact H.
       + now apply wf_EUnop.
   Qed.
-
-  Section ElaborateRecord.
-    Context (elaborate : tenv -> pexpr -> result {t & expr t}).
-
-    Fixpoint elaborate_record (G : tenv) (xs : list (string * pexpr)) :
-      result {t & expr t} :=
-      match xs with
-      | nil =>
-          Success (existT _ _ (EConst CEmpty))
-      | (s, p) :: xs =>
-          '(existT _ _ e1) <- elaborate G p;;
-          '(existT _ _ e2) <- elaborate_record G xs;;
-          Success (existT _ _ (EBinop (OPair s _ _) e1 e2))
-      end.
-  End ElaborateRecord.
 
   (* Type checks a `pexpr` and possibly emits a typed expression
      Checks scoping for variables/locations *)
@@ -347,8 +372,13 @@ Section WithMap.
         let G' := map.put G x (t1, false) in
         '(existT _ t2 e2) <- elaborate G' p2;;
         Success (existT _ _ (ELet x e1 e2))
-    | PERecord ps =>
-        elaborate_record elaborate G ps
+    | PERecord xs =>
+        let f '(s, p) :=
+          e <- elaborate G p;;
+          Success (s, e)
+        in
+        xs' <- List.all_success (List.map f xs);;
+        elaborate_record xs'
     | PEProj p s =>
       '(existT _ t e) <- elaborate G p;;
         elaborate_proj e s
@@ -493,35 +523,8 @@ Section WithMap.
       + now apply IHp1.
       + apply IHp2, H2.
     - (* PERecord xs *)
-      revert G t e H.
-      induction xs as [| [s p]]; intros G t e H.
-      + (* nil *)
-        inversion H. apply wf_EConst.
-      + (* (s, p) :: xs *)
-        unfold elaborate_record in H.
-        destruct (elaborate G p) as [[t1 e1] |] eqn : H1; try easy.
-        assert (elaborate_record elaborate G xs =
-          (fix elaborate_record
-             (G0 : tenv) (xs0 : list (string * pexpr)) {struct xs0} :
-               result {t0 : type & expr t0} :=
-             match xs0 with
-             | nil =>
-                 Success (existT (fun t0 : type => expr t0) TEmpty (EConst CEmpty))
-             | (s0, p1) :: xs1 =>
-                 ' (existT _ x e0) <- elaborate G0 p1;;
-                 ' (existT _ x0 e2) <- elaborate_record G0 xs1;;
-                 Success
-                   (existT (fun t0 : type => expr t0) (TPair s0 x x0)
-                      (EBinop (OPair s0 x x0) e0 e2))
-             end) G xs
-        ).
-        { easy. }
-        rewrite <- H0 in H. clear H0.
-        destruct (elaborate_record elaborate G xs) as [[t2 e2] |] eqn : H2; try easy.
-        inversion H.
-        apply wf_EBinop.
-        * apply elaborate_wf in H1. exact H1.
-        * apply IHxs. exact H2.
+      destruct List.all_success as [xs' |] eqn : H'; try easy.
+      now apply elaborate_record_wf with (xs := xs').
     - (* PEProj p s *)
       unfold elaborate_proj in H.
       destruct (elaborate G p) as [[t0 e0] |] eqn : H0; try easy.
